NFA

Reg.v
@@ -1,15 +1,22 @@
 Require Export Str.
-From mathcomp Require Export eqtype ssrnat.
-
+Unset Strict Implicit.
+Unset Printing Implicit Defensive.
 
 
 Inductive Reg : Σ -> Prop :=
-    | set0reg : Reg ∅
-    | emptyreg_ : Reg [set nil : finStr]
-    | set1reg (a : symbol) :  Reg [set ([:: a] : finStr)]   
-    | setUreg X Y : Reg X -> Reg Y -> Reg (X ∪ Y)
-    | setAreg X Y : Reg X -> Reg Y -> Reg (X ⋅ Y)
-    | setKreg X : Reg X -> Reg (X ^*).
+    | reg0 : Reg ∅
+    | regnil : Reg [set nil : finStr]
+    | rega (a : symbol) :  Reg [set ([:: a] : finStr)]   
+    | regU X Y : Reg X -> Reg Y -> Reg (X ∪ Y)
+    | regA X Y : Reg X -> Reg Y -> Reg (X ⋅ Y)
+    | regK X : Reg X -> Reg (X ^*).
+
+
+
+Record reg : Type := mkReg {
+    str :> Σ;
+    axiom :  Reg str
+}.
 
 
 Lemma cat1A (x y : finStr) :
@@ -31,43 +38,14 @@ Proof.
         move ->.
         rewrite cat1A; constructor => //; constructor.
     induction a0 => //.
-Qed.    
+Qed.  
 
 
-Lemma setDreg (R S : Σ) :
-    Reg R -> Reg S -> Reg (R // S).
-Proof.
-    move => HR HS; move : S HS.
-    rewrite -(set_enum R).
-    induction (enum R) => S HS.    
-    +   rewrite -enum_set0.
-        rewrite (set_enum ∅).
-        rewrite set0D; constructor.
-    +   rewrite set_cons setDUl; constructor.
-        -   Search set1 setD.
-            remember (a ∈ S).
-            destruct b.
-            *   suff : [set a] // S = ∅.
-                    move ->; constructor.
-                apply extension; apply /subsetP => x.
-                +   case /setDP.
-                    move /set1P ->.
-                    rewrite -Heqb => //.
-                +   rewrite (in_set0) => //.
-            *   have : [set a] // S = [set a].
-                    apply extension; apply /subsetP => b.
-                    +   case /setDP; move /set1P -> => _; apply /set1P => //.
-                    +   move /set1P ->; apply /setDP; split.
-                        -   apply /set1P => //.
-                        -   rewrite -Heqb => //.
-                move ->; apply reg1.
-        -   apply IHl => //.
-Qed.              
-
-Lemma setIreg : forall R S,
+Lemma regI : forall (R S : Σ),
     Reg R -> Reg S -> Reg (R ∩ S).
 Proof.
-    move => R S HR HS; move : S HS.
+    move => R S HR HS.
+    move : S HS => /=.
     rewrite -(set_enum R).
     induction (enum R) => S HS.
     +   rewrite -enum_set0.
@@ -89,7 +67,40 @@ Proof.
             *   rewrite (in_set0 x) => //.
 Qed.
 
-Lemma setTreg : Reg setT.
+
+
+
+Lemma regD (R S : Σ) :
+    Reg R -> Reg S -> Reg (R // S).
+Proof.
+    move => HR HS; move : S HS.
+    rewrite -(set_enum R).
+    induction (enum R) => S HS.    
+    +   rewrite -enum_set0.
+        rewrite (set_enum ∅).
+        rewrite set0D; constructor.
+    +   rewrite set_cons setDUl; constructor.
+        -   remember (a ∈ S).
+            destruct b.
+            *   suff : [set a] // S = ∅.
+                    move ->; constructor.
+                apply extension; apply /subsetP => x.
+                +   case /setDP.
+                    move /set1P ->.
+                    rewrite -Heqb => //.
+                +   rewrite (in_set0) => //.
+            *   have : [set a] // S = [set a].
+                    apply extension; apply /subsetP => b.
+                    +   case /setDP; move /set1P -> => _; apply /set1P => //.
+                    +   move /set1P ->; apply /setDP; split.
+                        -   apply /set1P => //.
+                        -   rewrite -Heqb => //.
+                move ->; apply reg1.
+        -   apply IHl => //.
+Qed.              
+
+
+Lemma regT : Reg setT.
 Proof.
     rewrite -(set_enum setT).
     induction (enum setT).
@@ -100,30 +111,44 @@ Proof.
         apply reg1.
 Qed.   
 
-Lemma setTDreg R : Reg R -> Reg (setT // R).
+Lemma regTD R : Reg R -> Reg (setT // R).
 Proof.
-    move => H; apply setDreg => //; apply setTreg.
+    move => H; apply regD => //; apply regT.
 Qed.
 
-Lemma setCreg R : Reg R -> Reg (¬ R).
+Lemma regC R : Reg R -> Reg (¬ R).
 Proof.
-    rewrite -setTD; apply setTDreg.
+    rewrite -setTD; apply regTD.
 Qed.
 
-Lemma setEreg R n :  Reg R -> Reg (R^n).
+
+Lemma regE R n :  Reg R -> Reg (R^n).
 Proof.
     induction n => /= H.
     +   apply reg1.
     +   constructor => //; apply IHn => //.
 Qed.
 
-Lemma setK'reg R : Reg R -> Reg (R^+).
+Lemma regK' R : Reg R -> Reg (R^+).
 Proof.
     move => H.
-    apply setDreg.
-    +   by apply setKreg.
+    apply regD.
+    +   by apply regK.
     +   by apply reg1.
-Qed.    
+Qed.
+
+
+
+
+
+
+
+
+
+
+
+
+
 
     
 
