Base.v
@@ -1,4 +1,4 @@
-From  mathcomp Require Export fintype ssrbool seq choice ssreflect finset.
+From mathcomp Require Export fintype ssrbool seq choice ssreflect finset.
 Unset Strict Implicit.
 Unset Printing Implicit Defensive.
 
@@ -11,6 +11,7 @@ Notation "A ⊂ B" := (A \subset B)(at level 30).
 Notation "A // B" := (setD A B)(at level 40).
 Notation "¬ A" := (setC A)(at level 40).
 Notation "pow[ A ]" := (powerset A).
+Notation "∅" := set0.
 
 Lemma extension {T : finType} (A B : {set T}) :
     A ⊂ B -> B ⊂ A -> A = B.
@@ -24,3 +25,13 @@ Lemma set_enum {T : finType} (A : {set T}) :
 Proof.
     by apply/setP => x; rewrite inE mem_enum .
 Qed.    
+
+Axiom bigcup : forall {T : finType}, {set {set T}} -> {set T}.
+Axiom bigcupP : forall {T : finType} (XX : {set {set T}}) (X : T),
+    reflect (exists (Y : {set T}), X ∈ Y /\ Y ∈ XX) (X ∈ bigcup XX).
+
+Axiom bigcap : forall {T : finType}, {set {set T}} -> {set T}.
+Axiom bigcapP : forall {T : finType} (XX : {set {set T}}) (X : T),
+    reflect (forall (Y : {set T}), Y ∈ XX -> X ∈ Y) (X ∈ bigcup XX).
+
+    
