NFA.v
@@ -1,0 +1,71 @@
+
+Require Export Str.
+
+
+
+Section NFA.
+
+
+Record sym : Type := mkSym {
+    symb :> finStr;
+    _ : symb ∈ ([set [::x]| x in [set : symbol]] ∪ [set ϵ]);
+}.
+
+
+
+Definition ϵ_ : sym.
+    apply (mkSym nil).
+    rewrite inE; apply /orP; right.
+    rewrite inE => //.
+Qed.
+
+Definition toSym (a : symbol) : sym.
+Proof.
+    apply (mkSym [:: a]).
+    rewrite inE; apply /orP; left.
+    apply /imsetP; exists a => //.
+Qed.
+
+
+Variable state : finType.
+Variables Q F : {set state}.
+Hypotheses FQ : F ⊂ Q.
+Variable p0 : state.
+Hypotheses pQ : p0 ∈ Q.
+Variable δ : state -> sym ->  {set state}.
+
+
+
+
+
+
+Reserved Notation "p -ϵ-> q"(at level 50).
+Inductive Closure : state -> state -> Prop :=
+    | CL_refl p : p -ϵ-> p
+    | CL_single p q : q ∈ δ p ϵ_ -> p -ϵ-> q
+    | CL_trans p q r : p -ϵ-> q -> q -ϵ-> r ->  p -ϵ-> r
+    where "p -ϵ-> q" := (Closure p q).
+
+Axiom closure : {set state} -> {set state}.
+Axiom closureP : forall (P : {set state}) q,
+    reflect (forall p, p ∈ P -> p -ϵ-> q) (q ∈ closure P).
+
+
+
+
+
+Fixpoint δ' (p : state) (s : finStr) : {set state} :=
+    match s with
+    | [::] => closure [set p]
+    | a :: w => closure (bigcup [set δ x (toSym a) | x in δ' p w])
+    end.
+
+Definition L := [set w : finStr | (δ' p0 w ∩ F) == ∅].
+
+
+End NFA.
+
+ 
+
+
+
